%++++++++++++++++++++++++++++++++++++++++
\documentclass[article,12pt]{article}
\usepackage{float}
\usepackage{setspace}
\usepackage{tabu} % extra features for tabular environment
\usepackage{amsmath}  % improve math presentation
\usepackage{graphicx} % takes care of graphic including machinery
\usepackage[margin=1in]{geometry} % decreases margins
\usepackage{cite} % takes care of citations
\usepackage[final]{hyperref} % adds hyper links inside the generated pdf file
\usepackage{tikz}
\usepackage{caption} 
\usepackage{fancyhdr}
\usepackage{amssymb} % symbols like /therefore
\usepackage{amsthm} % proofs
\usepackage{enumerate} % lettered lists
\usepackage{mathtools} % macros
\usetikzlibrary{scopes}
\usepackage{xcolor} \pagecolor[rgb]{0.12549019607,0.1294117647,0.13725490196} \color[rgb]{0.82352941176,0.76862745098,0.62745098039}
\hypersetup{
	colorlinks=true,       % false: boxed links; true: colored links
	linkcolor=blue,        % color of internal links
	citecolor=blue,        % color of links to bibliography
	filecolor=magenta,     % color of file links
	urlcolor=blue         
}

\newcounter{question}
\setcounter{question}{0}
\def\questionnum{{\Large\bfseries{Question \arabic{question} }}\\[1em]}

\newcommand{\question}{
    \stepcounter{question}
    \questionnum
}

\newcommand{\solution}{
    {{\large\bfseries{Solution}}}
}

\pagestyle{fancy}
\fancyhf{}% clears all header and footer fields
\fancyfoot[C]{--~\thepage~--}
\renewcommand*{\headrulewidth}{0pt}
\renewcommand*{\footrulewidth}{0pt}

\fancypagestyle{plain}{%
  \fancyhf{}% clears all header and footer fields
  \fancyfoot[C]{--~\thepage~--}%
  \renewcommand*{\headrulewidth}{0pt}%
  \renewcommand*{\footrulewidth}{0pt}%
}

% Shortcuts
\DeclarePairedDelimiter\ceil{\lceil}{\rceil}
\DeclarePairedDelimiter\floor{\lfloor}{\rfloor}
\DeclarePairedDelimiter\set{\{}{\}}
\DeclarePairedDelimiter\paren{(}{)}

\newcommand{\df}{\displaystyle\frac} % displaystyle fraction
\newcommand{\qeq}{\overset{?}{=}} % questionable equality

\newcommand{\xor}{\oplus}

\newcommand{\comp}{\circ}

\newcommand{\centervdots}{\mathrel{\makebox[\widthof{=}]{\vdots}}}

% Sets
\newcommand{\unite}{\cup}
\newcommand{\inter}{\cap}

\newcommand{\stcomp}[1]{\overline{#1}}  

\newcommand{\powset}{\mathcal{P}}
\newcommand{\reals}{\mathbb{R}} % real numbers: textbook is Z^+ and 0
\newcommand{\ints}{\mathbb{Z}}
\newcommand{\nats}{\mathbb{N}}
\newcommand{\rats}{\mathbb{Q}}

\setlength\parindent{0pt}

%++++++++++++++++++++++++++++++++++++++++

\title{Exam 2 Corrections}
\author{Denny Cao}
\date{%
    %CCP MATH163 \\%
    %Dr. Petrescu \\[2ex]%
    \today
}
\begin{document}
\maketitle

% Question 1
\question
If $\stcomp{A} \inter B = B \ \land \ \stcomp{B}\inter A = A$, what can you say about $A$ and $B$? Prove your answer. ($\stcomp{S}$ denotes the complement of $S$.) \\
\\
\solution
\begin{proof}
    Assume $x \in A$. By definition of complement, $x \notin \stcomp{A}$. Since $x \notin \stcomp{A}$, $x \notin \stcomp{A} \inter B$. Since $\stcomp{A} \inter B = B$, $x \notin B$. $x$ is arbitrary, therefore we can generalize to $A \not\subseteq{B}$.
\end{proof}
\begin{proof}
    Assume $y \in B$. By definition of complement, $y \notin \stcomp{B}$. Since $y \notin \stcomp{B}$, $y \notin \stcomp{B} \inter A$. Since $\stcomp{B} \inter A = A$, $y \notin A$. $y$ is arbitrary, therefore we can generalize to $B \not\subseteq A$.
\end{proof}
\begin{proof}
    Since $A \not\subseteq B \ \land \ B \not\subseteq A$, $A \inter B = \emptyset \\
    \\
    \stcomp{A} \inter B = B \ \land \ \stcomp{B} \inter A = A \implies A \inter B = \emptyset$
\end{proof}
\newpage
% Question 2
\question
Suppose that $g : A \rightarrow A$ and $f: A \rightarrow A$ where $A=\set*{a,b,c,d}$, $g=\set*{(a,a),(b,c),(c,a),(d,c)}$ and $f=\set*{(a,d),(b,a),(c,b),(d,a)}$. Find $g \comp (f \comp g)$, that is, find the composition of $g(x)$ with $f(x)$ composed with $g(x)$. \\
\\
\solution
\begin{align*}
    g &= \set*{(a,a),(b,c),(c,a),(d,c)} \\
    \\
    f \comp g &= f\paren*{\set*{(a,a),(b,c),(c,a),(d,c)}} \\
              &= \set*{(a,d),(b,b),(c,d),(d,b)} \\
    \\
    g \comp f \comp g &= g\paren*{\set*{(a,d),(b,b),(c,d),(d,b)}} \\
                      &= \set*{(a,c),(b,c),(c,c),(d,c)}
\end{align*}
\newpage
% Quesiton 3
\question 
Verify that $a_n = \pi$ \textbf{is a possible solution} to the recurrence relation $a_n = (2n-1)a_{n-1}-(2n-2)a_{n-2}$. What are the conditions for this to happen? \\
\\
\solution \\
Initial Conditions: $a_0 = \pi, a_1 = \pi$ 
\begin{align*}
    a_2 &= (2(2) - 1)a_1 - (2(2) - 2)a_0 \\
        &= 3a_1 - 2a_0 \\
        &= 3\pi - 2\pi \\
        &= \pi \\
    a_3 &= (2(3) - 1)a_2 - (2(3) - 2)a_1 \\
        &= 5a_2 - 4a_1 \\
        &= 5\pi - 4\pi \\
        &= \pi \\
    a_4 &= (2(4) - 1)a_3 - (2(4) - 2)a_2 \\
        &= 5a_3 - 4a_2 \\
        &= 5\pi - 4\pi \\
        &= \pi \\
    a_5 &= (2(5) - 1)a_4 - (2(5) - 2)a_3 \\
        &= 5a_4 - 4a_3 \\
        &= 5\pi - 4\pi \\
        &= \pi \\
        &\centervdots \\
    a_n &= (2n - 1)\pi - (2n - 2)\pi \\
        &= 2n\pi - \pi - 2n\pi + 2\pi \\
        &= \pi 
\end{align*}
Thus, the conditions for $a_n = \pi$ are $a_0 = \pi, a_1 = \pi$. 
\newpage
% Question 4
\question
Evaluate $\sum_{n=1}^{3}\sum_{k=1}^{n}(n^k)$. Show all your steps. \\
\\
\solution
\begin{align*}
    \sum_{n=1}^{3}\sum_{k=1}^{n}(n^k) &= \sum_{k=1}^{1}{1^k}+\sum_{k=1}^{2}{2^k}+ \sum_{k=1}^{3}{3^k} \\
                                      &= 1 + 2 + 4 + 3 + 9 + 27 \\
                                      &= 46
\end{align*}
\newpage
% Question 5
\question
Find a $f: \nats \rightarrow \ints$ that is surjection that is not injection. Prove that it satisfies the conditions held. \\
\\
\solution \\
$\nats = \ints^+ \unite \set*{0}$ \\
Suppose $S_1 = \set*{x \ | \ 2x, x \in \nats}$, $S_2 = \set*{x \ | \ 2x+1, x \in \nats}$
\[ f(x)=
\begin{cases}
    \frac{x}{2}                & x \in S_1 \\
    -(\frac{x}{2}-\frac{1}{2}) & x \in S_2 
\end{cases}
\]
\textbf{$f(n)$ is surjective.}
\begin{proof}
    We can separate the domain, $\nats$ into two sets of odd and even naturals, $S_1$ and $S_2$ respectively.
    \begin{align*}
    \intertext{Let $n=2y, y \in \nats$. Since $2y$ is an even integer, it will satisfy the first case, $x \in S_1$.}
        f(x)  &= \frac{x}{2}, x \in S_1 \\
        f(2y) &= \frac{2y}{2} \\
              &= y 
    \intertext{There exists an $x=2y$ that maps to all $\ints^+ \unite \set*{0}$ in the codomain.}
    \intertext{Let $n=2y + 1, y \in \nats$. Since $2y + 1$ is an odd integer, it will satisfy the second case, $x \in S_2$.}
        f(x)      &= -\paren*{\frac{x}{2} - \frac{1}{2}}, x \in S_2 \\
        f(2y + 1) &= -\paren*{\frac{2y + 1}{2} - \frac{1}{2}} \\
                  &= -\paren*{\frac{2y}{2}} \\
                  &= -y
    \intertext{There exists an $x=2y+1$ that maps to all $\ints^-$ in the codomain.}      
    \end{align*}
    Since $\ints^+ \unite \set*{0} \unite \ints^+ = \ints$, there exists an $x$ that maps to every value $y$ in the codomain. Thus, $f(x)$ is surjective. \\
\end{proof}
\newpage
\textbf{$f(n)$ is not injective.}
\begin{proof}
    Suppose $x_0 = 0, x_1 = 1$
    \begin{align*}
        f(x_0) &= \frac{0}{2} = 0 \\
        f(x_1) &= -\paren*{\frac{1}{2} - \frac{1}{2}} = 0
    \end{align*}
    Since there exists multiple values in the domain, $x_0, x_1$,  that map to the same value in the codomain, $0$, $f(x)$ is not injective. \\
\end{proof}
\newpage
% Question 6
\question
Suppose $\powset^n(A)$ = $\overbrace{\powset(\powset(\powset\cdots\powset(A))\cdots)}^{n}$, $n \in \ints^+$, where for instance, $\powset^3(A)=\powset(\powset(\powset(A)))$. Find the cardinality of $\powset^4(\emptyset)$, where $\powset(A)$ is the power set of $A$. \\
\\
\solution \\
The cardinality of the power set of a set is $2^n$, where $n$ is the cardinality of the set. \\
The cardinality of $\emptyset = 0$. 
\begin{alignat*}{5}
    &\powset(\emptyset)   &&= \set*{\emptyset} \ \ \                    &&|\powset(\emptyset)|   &&= 2^0 &&= 1 \\
    &\powset^2(\emptyset) &&= \set*{\emptyset, \set*{\emptyset}} \ \ \  &&|\powset^2(\emptyset)| &&= 2^1 &&= 2 \\
    &\powset^3(\emptyset) &&= \set*{\emptyset, \set*{\emptyset}, \set*{\set*{\emptyset}}, \set*{\emptyset, \set*{\emptyset}}} \ \ \ &&|\powset^3(\emptyset)| &&= 2^2 &&= 4 \\
\end{alignat*}
\[ |\powset^4(\emptyset)| = 16\]
\newpage
% Question 7
\question
Prove or disprove: $\forall$ sets $A,B,C, (A \xor B = A \xor C) \implies B=C$ \\
\\
\solution
\begin{proof} 
    \ \\
    \textbf{Case 1: Suppose $x \in B$} \\
    \textit{Subcase i: $x \in A$} \\
    $x \in B \land x \in A \implies x \notin A \xor B$. Since $A \xor B = A \xor C$, $x \notin A \xor C$. \\
    $x \in A \land x \notin A \xor C \implies x \in C$\\
    \\
    \textit{Subcase ii: $x \notin A$} \\
    $x \in B \land x \notin A \implies x \in A \xor B$. Since $A \xor B = A \xor C$, $x \in A \xor C$. \\
    $x \notin A \land x \in A \xor C \implies x \in C$ \\

    Since $x \in C$ in all cases when $x \in B$, $B \subseteq C$.\\
    \\
    \textbf{Case 2: Suppose $x \in C$} \\
    \textit{Subcase i: $x \in A$} \\
    $x \in C \land x \in A \implies x \notin A \xor C$. Since $A \xor C = A \xor B$, $x \notin A \xor B$. \\
    $x \in A \land x \notin A \xor B \implies x \in B$\\
    \\
    \textit{Subcase ii: $x \notin A$} \\
    $x \in C \land x \notin A \implies x \in A \xor C$. Since $A \xor C = A \xor B$, $x \in A \xor B$. \\
    $x \notin A \land x \in A \xor B \implies x \in B$ \\

    Since $x \in B$ in all cases when $x \in C$, $C \subseteq B$.\\
    \\
    $B \subseteq C \land C \subseteq B \implies B = C$. Thus, $(A \xor B = A \xor C) \implies B=C$. 
\end{proof}

\begin{align*}
    B &= \emptyset \xor B \\
      &= (A \xor A) \xor B \\
      &= A \xor (A \xor B) \\
      &= A \xor (A \xor C) \\
      &= (A \xor A) \xor C \\
      &= \emptyset \xor C \\
    B &= C
\end{align*}
\newpage
% Question 8
\question
Solve for $x$: $\floor*{2x} + \ceil*{2x} = 4x$ \\
\\
\solution \\
Any number can be represented by $a + b, a \in \ints, b \in \set*{k \ | \
 0 \leq k < 1}$. Let $x=a+b$. \\
\begin{align*}
    \floor*{2(a+b)} + \ceil*{2(a+b)}   &= 4(a+b) \\
    \floor*{2a + 2b} + \ceil*{2a + 2b} &= 4a + 4b \\ 
    2a + \floor*{2b} + 2a + \ceil*{2b} &= 4a + 4b \\
    \floor*{2b} + \ceil*{2b}           &= 4b 
\end{align*}
\begin{alignat*}{3}
\floor*{2b} =
\begin{cases}
    0 & 0 \leq b < 0.5 \\
    1 & 0.5 \leq b < 1 
\end{cases}
&& \ \ \ \ \ceil*{2b} =
\begin{cases}
    0 & b = 0 \\
    1 & 0 < b \leq 0.5 \\
    2 & 0.5 < b < 1
\end{cases}
\end{alignat*}
\begin{align*}
    4b &=
\begin{cases}
    0 + 0 = 0 \\
    0 + 1 = 1 \\
    1 + 1 = 2 \\
    1 + 3 = 3 
\end{cases} \\
b &= 
\begin{cases}
    \df{0}{4} \\[1em]
    \df{1}{4} \\[1em]
    \df{2}{4} \\[1em]
    \df{3}{4}
\end{cases}
\end{align*}
Thus, $x=a+b$, where $a \in \ints$ and $b \in \set*{\frac{1}{4}c \ | \ c \in 0 \leq c < 4, k \in \ints}$. Since all integers are multiples of $\frac{1}{4}$, $a$ can be represented as $a=\frac{1}{4}k, k \in \ints$. Since $b=\frac{1}{4}c, c \in 0 \leq c < 4, c \in \ints$, we can express $a+b$ as $\frac{1}{4}(k+c)$. Since $k$ and $c$ are both integers, $x$ is a multiple of $\frac{1}{4}$. \\
\begin{gather*}
    x \in \set*{\frac{1}{4}r \ | \ r \in \ints}
\end{gather*}
\newpage
\question
Give an example of two uncountable sets $A$ and $B$ such that $A \cap B$ is:\\a) finite. \hskip2.5cm b) countably infinite.\hskip2.5cm c) uncountable. \\
\\
\solution
\begin{enumerate}[(a)]
    \item 
        \begin{align*}
            A &= \reals^+ \unite \set*{0} \\
            B &= \reals^- \unite \set*{0}
        \end{align*}
        \begin{align*}
            A \inter B = \set*{0}
        \end{align*}
    \item 
        \begin{align*}
            A &= \reals^+ \unite \ints \\
            B &= \reals^- \unite \ints
        \end{align*}
        \begin{align*}
            A \inter B = \ints
        \end{align*}
    \item 
        \begin{align*}
            A &= \reals \\
            B &= \reals^+
        \end{align*}
        \begin{align*}
            A \inter B = \reals^+
        \end{align*}
\end{enumerate}
\newpage
\question
Prove if $f:A\rightarrow B$ and $g:B\rightarrow C$ are injective, then $g \comp f:A\rightarrow C$ is also injective. \\
\\
\solution
\begin{proof}
Suppose $x_0, x_1 \in A$. \\

Since $g$ is injective: 
\begin{align*}
    g(f(x_0)) = g(f(x_1)) \implies f(x_0) = f(x_1) 
\end{align*}
Since $f$ is injective:
\begin{align*}
    f(x_0) = f(x_1) \implies x_0 = x_1
\end{align*}
By Hypothetical Syllogism: 
\begin{align*}
    g(f(x_0)) = g(f(x_1)) \implies x_0 = x_1
\end{align*}
Thus, $\forall x_0 \forall x_1 (g(f(x_0)) = g(f(x_1)) \implies x_0 = x_1)$. Therefore, $g \comp f$ is injective.    
\end{proof}
\end{document} 

